

Exercise 5.1.

- 1) Show that i is a double root of $P(x) = x^6 + x^5 + 3x^4 + 2x^3 + 3x^2 + x + 1$.
- 2) Factor P in $\mathbb{C}[x]$ and in $\mathbb{R}[x]$.

Exercise 5.2.

Find a polynomial of degree 3 which admits two simple roots $x_0 = 1$ and $x_1 = 2$ and that the remainder of its Euclidean division by $x^2 + 1$ is $R(x) = 1$.

Exercise 5.3.

1. Perform the Euclidean division of P by Q
 - (a) $P = 3x^4 + 3x^2 + 1, Q = x^2 + 2x + 3 - 1$
2. Perform the division in ascending powers of P by Q to the order k .
 - (a) $P = 1 - 2x + x^3 + x^3, Q = 2 + 2x + x^2, k = 3$.

Exercise 5.4.

Let P and $Q \in \mathbb{R}[x]$ two polynomials such that $P(x) = x^4 - 5x^3 + 4x^2 - 3x + 3$ and $Q(x) = x^3 - x^2 - x + 1$.

- 1) Find D the greatest common divisor of P and Q .
- 2) Find U and V two polynomials of $\mathbb{R}[x]$ such that $PU + QV = D$.

Exercise 5.5.

Let P be a polynomial of $\mathbb{R}[x]$ such that $P(i) = 0$.

- 1) Show that there exists a polynomial Q of $\mathbb{R}[x]$ verifying $\forall x \in \mathbb{R} : P(x) = (x^2 + 1)Q(x)$.
- 2) Factor $P(x) = x^5 + x^3 - x^2 - 1$ in $\mathbb{C}[x]$ and in $\mathbb{R}[x]$.

Exercise 5.6.

Let $n \in \mathbb{N}$ and P, Q two polynomials in $\mathbb{R}[x]$ such that :

$$P(x) = (x - 1)^{n+2} + x^{2n+1} + 1 \text{ and } Q(x) = x^2 - x + 1.$$

- 1) Show that $-j$ is a root of Q .
- 2) Calculate $P(-j)$.
- 3) Deduce the remainder of the division of P by Q .

Exercise 5.7.

Let $P(x) = 2x^3 + x^2 + x - 1 \in \mathbb{R}[x]$.

- 1) Show that, if P admits a rational root written under irreducible form $\frac{a}{b}$ then $a|1$ and $b|2$.
- 2) Deduce all rational roots of P .
- 3) Find all roots of P in \mathbb{R} .

Exercise 5.8.

A Let $P(x) = x^5 + 4x^3 - x^2 - 4 \in \mathbb{R}[x]$.

- 1) Verify that the complex numbers $2i$ and j are roots of the polynomial P .
- 2) Find the other two complex roots of P .
- 3) Factor P into irreducible factors in $\mathbb{C}[x]$ then in $\mathbb{R}[x]$.

B Let $Q(x) = x^{6n+2} + x^{3n+1} + 1 \in \mathbb{R}[x], n \in \mathbb{N}^*$.

- 1) Verify that j is a root of Q .
- 2) For $n = 1$, give two polynomials Q_1, Q_2 in $\mathbb{R}[x]$ such that $Q = Q_1Q_2$ with $d^\circ Q_1 = 2$ and $d^\circ Q_2 = 6$.

1 Solutions

Solution to exercise 3.1.

- 1) We have: $P(i) = 0$, $P'(i) = 0$ and $P''(i) \neq 0$. Then i is a double root of P .
- 2) Since i is a double root of P and $P \in \mathbb{R}[x]$ then $-i$ is a double root of P so we can write P in the form:

$$P(x) = (x - i)^2 (x + i)^2 Q(x) \text{ where } (d^\circ Q = 2).$$

We can deduce Q using the Euclidean division of $P(x)$ by $(x^2 + 1)^2$. We get:

$$\begin{array}{r|l} \begin{array}{r} x^6 + x^5 + 3x^4 + 2x^3 + 3x^2 + x + 1 \\ -(x^6 + 2x^4 + x^2) \\ \hline x^5 + x^4 + 2x^3 + 2x^2 + x + 1 \\ -(x^5 + 2x^3 + x) \\ \hline x^4 + 2x^2 + 1 \\ -(x^4 + 2x^2 + 1) \\ \hline 0 \end{array} & \frac{x^4 + 2x^2 + 1}{x^2 + x + 1} \end{array}$$

then $Q(x) = x^2 + x + 1$. The roots of Q are j and j^2 then factoring Q into $\mathbb{C}[x]$ is:

$$P(x) = (x - i)^2 (x + i)^2 (x - j) (x - j^2) \text{ où } (j = -\frac{1}{2} + \frac{\sqrt{3}}{2}i)$$

and factoring Q into $\mathbb{R}[x]$ is:

$$P(x) = (x^2 + 1)^2 (x^2 + x + 1)$$

because the polynomials $x^2 + 1$ and $x^2 + x + 1$ are irreducible in $\mathbb{R}[x]$.

Solution de l'exercice 3.1.

- 1) We have: $P(i) = 0$, $P'(i) = 0$ and $P''(i) \neq 0$. Then i is a double root of P .
- 2) Since i is a double root of P and $P \in \mathbb{R}(x)$ then $-i$ is a double root of P so we can éwrite P in the form:

$$P(x) = (x - i)^2 (x + i)^2 Q(x) \text{ où } (d^\circ Q = 2).$$

We can deduce Q using the Euclidean division of $P(x)$ by $(x^2 + 1)^2$. We obtain:

$$\begin{array}{r|l} \begin{array}{r} x^6 + x^5 + 3x^4 + 2x^3 + 3x^2 + x + 1 \\ -(x^6 + 2x^4 + x^2) \\ \hline x^5 + x^4 + 2x^3 + 2x^2 + x + 1 \\ -(x^5 + 2x^3 + x) \\ \hline x^4 + 2x^2 + 1 \\ -(x^4 + 2x^2 + 1) \\ \hline 0 \end{array} & \frac{x^4 + 2x^2 + 1}{x^2 + x + 1} \end{array}$$

then $Q(x) = x^2 + x + 1$. The roots of Q are j and j^2 then factoring Q into $\mathbb{C}[x]$ is:

$$P(x) = (x - i)^2 (x + i)^2 (x - j) (x - j^2) \text{ où } (j = -\frac{1}{2} + \frac{\sqrt{3}}{2}i)$$

and factoring Q into $\mathbb{R}[x]$ is:

$$P(x) = (x^2 + 1)^2 (x^2 + x + 1)$$

because the polynomials $x^2 + 1$ and $x^2 + x + 1$ are irreducible in $\mathbb{R}[x]$.

Solution to exercise 3.1.

- 1) We have: $P(i) = 0$, $P'(i) = 0$ and $P''(i) \neq 0$. Then i is a double root of P .
- 2) Since i is a double root of P and $P \in \mathbb{R}(x)$ then $-i$ is a double root of P so we can éwrite P in the form:

$$P(x) = (x - i)^2 (x + i)^2 Q(x) \text{ où } (d^\circ Q = 2).$$

We can deduce Q using the Euclidean division of $P(x)$ by $(x^2 + 1)^2$. We obtain:

$$\begin{array}{r|l} \begin{array}{r} x^6 + x^5 + 3x^4 + 2x^3 + 3x^2 + x + 1 \\ -(x^6 + 2x^4 + x^2) \\ \hline x^5 + x^4 + 2x^3 + 2x^2 + x + 1 \\ -(x^5 + 2x^3 + x) \\ \hline x^4 + 2x^2 + 1 \\ -(x^4 + 2x^2 + 1) \\ \hline 0 \end{array} & \frac{x^4 + 2x^2 + 1}{x^2 + x + 1} \end{array}$$

then $Q(x) = x^2 + x + 1$. The roots of Q are j and j^2 then factoring Q into $\mathbb{C}[x]$ is:

$$P(x) = (x - i)^2 (x + i)^2 (x - j) (x - j^2) \text{ where } (j = -\frac{1}{2} + \frac{\sqrt{3}}{2}i)$$

and factoring Q into $\mathbb{R}[x]$ is:

$$P(x) = (x^2 + 1)^2 (x^2 + x + 1)$$

because the polynomials $x^2 + 1$ and $x^2 + x + 1$ are irreducible in $\mathbb{R}[x]$.

Solution to exercise 3.2.

Since the remainder of the Euclidean division of $P(x)$ by $x^2 + 1$ is 1, then $\exists (a, b) \in \mathbb{R}^2$ such that:

$$P(x) = (ax + b)(x^2 + 1) + 1$$

then 1 and 2 are roots of P , therefore:

$$\begin{cases} (a + b)(1^2 + 1) + 1 = 0 \\ (2a + b)(2^2 + 1) + 1 = 0 \end{cases} \Rightarrow \begin{cases} a = \frac{3}{10} \\ b = -\frac{4}{5} \end{cases}.$$

SO

$$\begin{aligned} P(x) &= \left(\frac{3}{10}x + -\frac{4}{5} \right) (x^2 + 1) + 1 \\ &= \frac{3}{10}x^3 - \frac{4}{5}x^2 + \frac{3}{10}x + \frac{1}{5}. \end{aligned}$$

Solution to exercise 3.3.

1) We have:

$$\left. \begin{array}{l} x^4 - 5x^3 + 4x^2 - 3x + 3 \\ -(x^4 - x^3 - x^2 + x) \\ \hline -4x^3 + 5x^2 - 4x + 3 \\ -(-4x^3 + 4x^2 + 4x - 4) \\ \hline x^2 - 8x + 7 \end{array} \right| \frac{x^3 - x^2 - x + 1}{x - 4}.$$

From where ' $P(x) = (x - 4)Q(x) + (x^2 - 8x + 7)$ ', then we have:

$$\left. \begin{array}{l} x^3 - x^2 - x + 1 \\ -(x^3 - 8x^2 + 7x) \\ \hline 7x^2 - 8x + 1 \\ -(7x^2 - 56x + 49) \\ \hline 48x - 48 \end{array} \right| \frac{x^2 - 8x + 7}{x + 7}.$$

So $Q(x) = (x^2 - 8x + 7)(x + 7) + 48x - 48$. We have:

$$\left. \begin{array}{l} x^2 - 8x + 7 \\ -(x^2 - x) \\ \hline -7x + 7 \\ -(-7x + 7) \\ \hline 0 \end{array} \right| \frac{48x - 48}{\frac{1}{48}x - \frac{7}{48}}$$

Then $D = \gcd(P, Q) = x - 1$.

2) We have:

$$x - 1 = \frac{1}{48}Q(x) - \frac{1}{48}(x^2 - 8x + 7)(x + 7)$$

And

$$(x^2 - 8x + 7) = P(x) - (x - 4)Q(x)$$

SO

$$x - 1 = \frac{1}{48}Q(x) - \frac{1}{48}(P(x) - (x - 4)Q(x))(x + 7).$$

SO

$$x - 1 = \frac{1}{48}(1 + (x - 4)(x + 7))Q(x) - \frac{1}{48}(x + 7)P(x),$$

hence $U(x) = -\frac{1}{48}(x + 7)$ and $V(x) = \frac{1}{48}(x^2 + 3x - 27)$.

Solution to exercise 3.4.

-
- 1) We have: $P(x) \in \mathbb{R}[x]$ and $P(i) = 0$ then $P(-i) = 0$. So we can factor P in $\mathbb{C}[x]$ as follows:

$$P(x) = (x+i)(x-i)Q(x) \text{ with } Q(x) \in \mathbb{C}[x].$$

Hence $P(x) = (x^2 + 1)Q(x)$.

* We show that $Q(x) \in \mathbb{R}[x]$. We have: $\overline{P(x)} = P(\bar{x})$, therefore

$$\overline{(x^2 + 1)Q(x)} = (\bar{x}^2 + 1)Q(\bar{x}) \Rightarrow (\bar{x}^2 + 1)\overline{Q(x)} = (\bar{x}^2 + 1)Q(\bar{x})$$

it therefore follows that $\overline{Q(x)} = Q(\bar{x})$. Then $Q(x) \in \mathbb{R}[x]$.

- 2) We have: $P(i) = 0$, then we can factor P as follows:

$$P(x) = (x^2 + 1)(x^3 - 1)$$

so $P(x) = (x-i)(x+i)(x-1)(x-j)(x-j^2)$ in $\mathbb{C}[x]$,

and $P(x) = (x^2 + 1)(x-1)(x^2 + x + 1)$ in $\mathbb{R}[x]$.

Solution to exercise 3.5.

- 1) Like $j^2 = -j - 1$, therefore

$$Q(-j) = j^2 + j + 1 = 0$$

hence $-j$ is a root of Q .

- 2) We have: $P(-j) = (-j-1)^{n+2} + (-j)^{2n+1} + 1$ is like $-j-1 = j^2$, so

$$\begin{aligned} P(-j) &= j^{2n+4} - j^{2n+1} + 1 \\ &= j^{2n+1} - j^{2n+1} + 1 = 0 \end{aligned}$$

hence $P(-j) = 1$.

- 3) We assume that:

$$P(x) = Q(x)U(x) + R(x) \text{ with } d^\circ(R) < d^\circ(Q)$$

hence $R(x) = ax + b$ with $(a, b) \in \mathbb{R}^2$. As $P(-j) = 0$ then $R(-j) = 1$ therefore $R(x) = 1$.

Solution to exercise 3.6.

- 1) P admits a rational root written in form irreducible $\frac{a}{b}$ then:

$$\begin{aligned} P\left(\frac{a}{b}\right) = 0 &\Rightarrow 2\left(\frac{a}{b}\right)^3 + \left(\frac{a}{b}\right)^2 + \frac{a}{b} - 1 = 0 \\ &\Rightarrow a(2a^2 + ba + b^2) = b^3 \\ &\Rightarrow a|b^3 \end{aligned}$$

like $a \wedge b = 1$ then according to the Gaussian theorem we have $a|1$. Then we have:

$$\begin{aligned} 2\left(\frac{a}{b}\right)^3 + \left(\frac{a}{b}\right)^2 + \frac{a}{b} - 1 = 0 &\Rightarrow 2a^3 = b(b^2 - a^2 - ab) \\ &\Rightarrow b|2a^3 \end{aligned}$$

like $a \wedge b = 1$ then according to the Gaussian theorem we have $b|2$.

2) If $\frac{a}{b}$ is a root of P , then $a \in \{-1, 1\}$ and $b \in \{-1, -2, 1, 2\}$ from where

$$\frac{a}{b} \in \left\{-1, 1, -\frac{1}{2}, \frac{1}{2}\right\}.$$

Like $P(-1) \neq 0$, $P(1) \neq 0$, $P(-\frac{1}{2}) \neq 0$ and $P(\frac{1}{2}) = 0$, then $\frac{1}{2}$ is a rational root of P .

3) As $\frac{1}{2}$ is a root of P then we can rewrite P in the form:

$$\begin{aligned} P(x) &= \left(x - \frac{1}{2}\right) (ax^2 + bx + c) \\ &= ax^3 + \left(b - \frac{1}{2}a\right)x^2 + \left(c - \frac{1}{2}b\right)x - \frac{1}{2}c. \end{aligned}$$

By identification, we obtain:

$$a = 2, b = 2 \text{ and } c = 2.$$

Hence the other roots are the roots of polynomial $2(x + x^2 + 1)$ i.e. j and j^2 .

Solution to exercise 3.7.

A/ 1) We have: $P(2i) = 0$, $P(j) = 0$.

2) Since $P \in \mathbb{R}[x]$ then the other two complex roots of P are $-2i$ and \bar{j} .

3) We have:

$$P(x) = (x - i)(x + i)(x - j)(x - \bar{j})(ax + b)$$

so by identification we obtain : $a = 1$ and $b = -1$ therefore

$$P(x) = (x - 2i)(x + 2i)(x - j)(x - \bar{j})(x - 1).$$

Then factoring P into $\mathbb{R}[x]$ is:

$$P(x) = (x^2 + 4)(x^2 + x + 1)(x - 1).$$

B/ We have: $Q \in \mathbb{R}[x]$, $n \in \mathbb{N}^*$.

1) We have:

$$\begin{aligned} Q(j) &= j^{6n+2} + j^{3n+1} + 1 \\ &= j \times j^{6n} + j^{3n} \times j + 1 \\ &= j^2 + j + 1 = 0 \end{aligned}$$

therefore j is a root of Q .

2) For $n = 1$, $Q(x) = x^8 + x^4 + 1$ and since j is a root of Q and $Q(-x) = Q(x)$ then:

$$Q(j) = Q(\bar{j}) = 0.$$

Hence:

$$\begin{aligned} Q(x) &= (x - j)(x - \bar{j})Q_2(x), \text{ with } d^\circ Q_2 = 6 \\ &= (x^2 + x + 1)Q_2(x). \end{aligned}$$

By Euclidean division we obtain:

$$\begin{array}{r|l}
\begin{array}{r}
x^8 + x^4 + 1 \\
-(x^8 + x^7 + x^6) \\
\hline
-x^7 - x^6 + x^4 + 1 \\
-(-x^7 - x^6 - x^5) \\
\hline
x^5 + x^4 + 1 \\
-(x^5 + x^4 + x^3) \\
\hline
-x^3 + 1 \\
-(-x^3 - x^2 - x) \\
\hline
x^2 + x + 1 \\
-(x^2 + x + 1) \\
\hline
0
\end{array}
&
\begin{array}{l}
\frac{x^2 + x + 1}{x^6 - x^5 + x^3 - x + 1}
\end{array}
\end{array}$$

$$Q_2(x) = x^6 - x^5 + x^3 - x + 1.$$